Merged quic2c into new-master.

apps/cmitls/cmitls.c
@@ -191,10 +191,10 @@ mitls_nego_action nego_callback(void *cb_state, mitls_version ver,
   printf(" @@@@ Nego callback for %s @@@@\n", pvname(ver));
   printf("Offered extensions:\n");
   dump(cexts, cexts_len);
-
+  
   unsigned char *qtp = NULL;
   size_t qtp_len;
-  if(FFI_mitls_find_custom_extension(option_isserver, cexts, cexts_len, (uint16_t)0x1A, &qtp, &qtp_len))
+  if(FFI_mitls_find_custom_extension(1, cexts, cexts_len, (uint16_t)0x1A, &qtp, &qtp_len))
   {
     printf("Transport parameters:\n");
     dump(qtp, qtp_len);
@@ -336,6 +336,7 @@ int ConfigureQuic(quic_state **pstate)
     };
 
     memset(&quic_cfg, 0, sizeof(quic_cfg));
+    quic_cfg.callback_state = pstate;
     quic_cfg.is_server = (option_isserver) ? 1 : 0;
     quic_cfg.cipher_suites = option_ciphers;
     quic_cfg.cert_callbacks = &cert_callbacks;
@@ -536,7 +537,7 @@ int SingleServer(mitls_state *state, SOCKET clientfd)
     strcat(payload, ctext);
     strncat(payload, (const char*)db, db_length);
 
-    FFI_mitls_free_packet(state, db);
+    FFI_mitls_free(state, db);
     r = FFI_mitls_send(state, (unsigned char*)payload, strlen(payload));
     if (r == 0) {
         printf("FFI_mitls_send() failed\n");
@@ -775,7 +776,7 @@ int SingleQuicServer(quic_state *state, SOCKET clientfd)
     quic_recv_until(state, clientfd, check_true);
     quic_dump(state);
 
-    FFI_mitls_quic_free(state);
+    FFI_mitls_quic_close(state);
     return 0;
 }
 
@@ -919,7 +920,7 @@ int TestClient(void)
       // otherwise, don't.
       if (!*option_file)
         puts((const char *)response);
-      FFI_mitls_free_packet(state, response);
+      FFI_mitls_free(state, response);
       // JP: TODO: how to determine when we have nothing left to read?
       if (response_length < 16384)
         break;
